progress in safek preservation, leave the problem of different choice of outgoing world in different k

common/Invariant.v
@@ -139,6 +139,17 @@ Qed.
 
 (** * Calling conventions as invariants *)
 
+Definition invcc {liA liB} (IA: invariant liA) (cc: callconv liA liB) : invariant liB :=
+  {|
+    inv_world := (inv_world IA * ccworld cc);
+    symtbl_inv '(wA, wcc) se2 := exists se1, symtbl_inv IA wA se1
+                                        /\ match_senv cc wcc se1 se2;
+    query_inv '(wA, wcc) q2 := exists q1, query_inv IA wA q1
+                                     /\ match_query cc wcc q1 q2; 
+    reply_inv '(wA, wcc) r2 := exists r1, reply_inv IA wA r1 /\ match_reply cc wcc r1 r2;
+  |}.
+
+
 Definition invcc_in {liA liB} (IA: invariant liA) (cc: callconv liA liB) : invariant liB :=
   {|
     inv_world := (inv_world IA * ccworld cc);
